Add random grid generation

sumplete/sumplete.dfy
@@ -5,89 +5,103 @@ Project: Part 1 - Sumplete
 
 module DataStructure {
   /**
-  Sums of a grid.
-   */
-  class Sums {
-    var rows: array<int>
-    var columns: array<int>
-
-    constructor(size: nat)
-      ensures rows.Length == size
-      ensures columns.Length == size
-    {
-      rows := new int[size];
-      columns := new int[size];
-    }
-
-    method updateRows(sums: array<int>)
-      modifies this
-      requires sums.Length == rows.Length
-    {
-      rows := sums;
-    }
-
-    method updateColumns(sums: array<int>)
-      modifies this
-      requires sums.Length == columns.Length
-    {
-      columns := sums;
-    }
-
-    /*
-    function rowsMatch(playerRows: array<int>) : (matches: bool)
-      reads playerRows
-      reads this
-      requires rows.Length == playerRows.Length
-      ensures forall i | 0 <= i < rows.Length :: rows[i] == playerRows[i] ==> matches == true
-      ensures exists i | 0 <= i < rows.Length :: rows[i] != playerRows[i] ==> matches == false
-    {
-      // TODO
-    }
-    */
-  }
-
-  /**
   The sumplete grid.
    */
   class Grid {
     // n*n grid -> rows*columns
-    var grid_start: array2<int>
-    var sum_target: Sums
+    var start_grid: array2<int>
+    var target_grid: array2<int>
+    var target_rows_sum: array<int>
+    var target_columns_sum: array<int>
 
-    var grid_player: array2<int>
-    var sum_player: Sums
+    // n*n grid -> rows*columns
+    var player_grid: array2<int>
+    var player_rows_sum: array<int>
+    var player_columns_sum: array<int>
 
-    constructor(grid: array2<int>)
-      requires grid.Length0 == grid.Length1
-      ensures grid_start.Length0 == grid_start.Length1
-      ensures grid_start.Length0 == grid_player.Length0
-      ensures grid_start.Length1 == grid_player.Length1
-      ensures grid_start.Length0 == sum_target.rows.Length
-      ensures grid_player.Length0 == sum_player.rows.Length
+    predicate Valid()
+      reads this
+      reads start_grid
+      reads target_grid, target_rows_sum, target_columns_sum
+      reads player_grid, player_rows_sum, player_columns_sum
     {
-      grid_start := grid;
-      grid_player := new int[grid.Length0, grid.Length1]((i, j) => 0);
+      // ensure n*n grid
+      start_grid.Length0 == start_grid.Length1 &&
 
-      sum_target := new Sums(grid.Length0);
-      sum_player := new Sums(grid.Length0);
+      // ensure start_grid, target_grid and player_grid have the same size
+      start_grid.Length0 == target_grid.Length0 && start_grid.Length1 == target_grid.Length1 &&
+      start_grid.Length0 == player_grid.Length0 && start_grid.Length1 == player_grid.Length1 &&
+
+      // ensure sum arrays have same length as rows & columns
+      start_grid.Length0 == target_rows_sum.Length && start_grid.Length1 == target_columns_sum.Length &&
+      player_grid.Length0 == target_rows_sum.Length && player_grid.Length1 == target_columns_sum.Length
+    }
+
+    constructor(size: int)
+      requires size > 0
+      ensures Valid()
+    {
+      start_grid := new int[size, size]((i, j) => 0);
+      target_grid := new int[size, size]((i, j) => 0);
+      target_rows_sum := new int[size](i => 0);
+      target_columns_sum := new int[size](i => 0);
+
+      player_grid := new int[size, size]((i, j) => 0);
+      player_rows_sum := new int[size](i => 0);
+      player_columns_sum := new int[size](i => 0);
+    }
+
+    method setupGame()
+      modifies this, start_grid, target_grid, target_rows_sum, target_columns_sum
+      requires Valid()
+      ensures Valid()
+    {
+      var i, j := 0, 0;
+      var size := start_grid.Length0;
+
+      while i < size
+        invariant size == start_grid.Length0
+        invariant Valid()
+        modifies start_grid, target_grid
+      {
+        while j < size
+          invariant size == start_grid.Length0
+          invariant Valid()
+          modifies start_grid, target_grid
+        {
+          start_grid[i,j] := random();
+          var randomBool := randomBool();
+          if randomBool {
+            target_grid[i,j] := start_grid[i,j];
+          }
+          j := j + 1;
+        }
+        i := i + 1;
+      }
     }
 
     /**
-    Sets the row or column sum.
-     */
-    /*
-    method setSums(rowSums: array<int>, columnSums: array<int>)
-      modifies this
-      requires rowSums.Length == sum_target.rows.Length
-      requires columnSums.Length == sum_target.columns.Length
+    Random number generator.
+    */
+    method random() returns (randomNumber: nat)
+      ensures 1 <= randomNumber <= 9
     {
-      sum_target.updateRows(rowSums);
-      sum_target.updateColumns(columnSums);
-    }*/
+      var numberSet := {1, 2, 3, 4, 5, 6, 7, 8, 9};
+      randomNumber :| randomNumber in numberSet;
+    }
+
+    /**
+    Random boolean generator.
+    */
+    method randomBool() returns (randomBool: bool)
+    {
+      var bools: set<bool> := {true, false};
+      randomBool :| randomBool in bools;
+    }
   }
 }
 
-module GameSetup {
+module Game {
   import dataStructure = DataStructure
 
   /**
@@ -96,70 +110,6 @@ module GameSetup {
   method setupGame(size: nat) returns (grid: dataStructure.Grid)
     requires size > 0
   {
-    var newGrid := createRandomGridOfSize(size);
-    grid := new dataStructure.Grid(newGrid);
-
-    var solutionGrid := createRandomSolutionGrid(newGrid);
-  }
-
-  /**
-  Creates a grid of size, with random numbers in every cell.
-   */
-  method createRandomGridOfSize(size: nat) returns (grid: array2<int>)
-    ensures grid.Length0 == grid.Length1
-  {
-    grid := new int[size, size]((i, j) => 0);
-
-    var i := 0;
-    var j := 0;
-    while i < grid.Length0 {
-      while j < grid.Length1 {
-        grid[i,j] := random();
-        j := j+1;
-      }
-      i := i+1;
-    }
-  }
-
-  /**
-  Creates a grid that only includes the numbers that should be counted to the column and row sums.
-   */
-  method createRandomSolutionGrid(grid: array2<int>) returns (solutionGrid: array2<int>)
-  {
-    solutionGrid := new int[grid.Length0, grid.Length1]((i, j) => 0);
-    var i := 0;
-    var j := 0;
-    var shouldBeCounted := false;
-    while i < solutionGrid.Length0 {
-      while j < solutionGrid.Length1 {
-        shouldBeCounted := randomBool();
-        if shouldBeCounted {
-          solutionGrid[i,j] := grid[i,j];
-        } else {
-          solutionGrid[i,j] := 0;
-        }
-        j := j+1;
-      }
-      i := i+1;
-    }
-  }
-
-  /**
-  Random number generator.
-   */
-  method random() returns (randomNumber: nat)
-    ensures 1 <= randomNumber <= 9
-  {
-    var numberSet := {1, 2, 3, 4, 5, 6, 7, 8, 9};
-    randomNumber :| randomNumber in numberSet;
-  }
-
-  /**
-  Random boolean generator.
-   */
-  method randomBool() returns (randomBool: bool)
-  {
-    var bools: set<bool> := {true, false};
-    randomBool :| randomBool in bools;
+    grid := new dataStructure.Grid(size);
   }
 }
